CoqOfRust/ink/ink_primitives.v
@@ -61,7 +61,7 @@ Module types.
   Module Clear.
     Class Trait (Self : Set) : Type := {
       CLEAR_HASH `{H' : State.Trait} : Self;
-      is_clear `{H' : State.Trait} : (ref Self) -> (M (H := H') bool);
+      is_clear `{H' : State.Trait} : (ref Self) -> M (H := H') bool;
     }.
     
     Global Instance Method_CLEAR_HASH `{H' : State.Trait} `(Trait)
@@ -117,7 +117,7 @@ Definition Hash := @Hash.t.
 Module Clear.
   Class Trait (Self : Set) : Type := {
     CLEAR_HASH `{H' : State.Trait} : Self;
-    is_clear `{H' : State.Trait} : (ref Self) -> (M (H := H') bool);
+    is_clear `{H' : State.Trait} : (ref Self) -> M (H := H') bool;
   }.
   
   Global Instance Method_CLEAR_HASH `{H' : State.Trait} `(Trait)
