coq_translation/default/examples/functions/functions_order.v
@@ -48,8 +48,8 @@ End Impl_functions_order_SomeType.
 
 Module SomeTrait.
   Class Trait (Self : Set) : Type := {
-    some_trait_foo `{H' : State.Trait} : (ref Self) -> (M (H := H') unit);
-    some_trait_bar `{H' : State.Trait} : (ref Self) -> (M (H := H') unit);
+    some_trait_foo `{H' : State.Trait} : (ref Self) -> M (H := H') unit;
+    some_trait_bar `{H' : State.Trait} : (ref Self) -> M (H := H') unit;
   }.
   
   Global Instance Method_some_trait_foo `{H' : State.Trait} `(Trait)
