coq_translation/default/examples/traits/disambiguating_overlapping_traits.v
@@ -3,7 +3,7 @@ Require Import CoqOfRust.CoqOfRust.
 
 Module UsernameWidget.
   Class Trait (Self : Set) : Type := {
-    get `{H' : State.Trait} : (ref Self) -> (M (H := H') alloc.string.String);
+    get `{H' : State.Trait} : (ref Self) -> M (H := H') alloc.string.String;
   }.
   
   Global Instance Method_get `{H' : State.Trait} `(Trait)
@@ -14,7 +14,7 @@ End UsernameWidget.
 
 Module AgeWidget.
   Class Trait (Self : Set) : Type := {
-    get `{H' : State.Trait} : (ref Self) -> (M (H := H') u8);
+    get `{H' : State.Trait} : (ref Self) -> M (H := H') u8;
   }.
   
   Global Instance Method_get `{H' : State.Trait} `(Trait)
